\documentclass[11pt]{article}
\usepackage{fullpage}

\begin{document}



question 5\\

\textbf{Wrong Answer}

\begin{tabular}{|c|c|c|c|c|c|c|}
\hline 
p & q & r & $p \rightarrow q$ (2) & $ (2) \rightarrow R$ & $P \land \neg Q$ (3) & (3) $\lor R$ \\ 
\hline 
1 & 1 & 1 & 1 & 1 & 0 & 1 \\ 
\hline 
1 & 1 & 0 & 1 & 0 & 0 & 0 \\ 
\hline 
1 & 0 & 1 & 0 & 1 & 1 & 1 \\ 
\hline 
0 & 0 & 0 & 0 & 0 & 0 & 0 \\ 
\hline 
0 & 1 & 1 & 1 & 1 & 0 & 1 \\ 
\hline 
0 & 1 & 0 & 1 & 0 & 0 & 0 \\ 
\hline 
• & • & • & • & • & • & • \\ 
\hline 
• & • & • & • & • & • & • \\ 
\hline 
\end{tabular} \\

\textbf{Correct Table}

\begin{tabular}{|c|c|c|c|c|c|c|}
\hline 
p & q & r & $p \rightarrow q$ (2) & $ (2) \rightarrow R$ & $P \land \neg Q$ (3) & (3) $\lor R$ \\ 
\hline 
1 & 1 & 1 & 1 & 1 & 0 & 1 \\ 
\hline 
1 & 1 & 0 & 1 & 0 & 0 & 0 \\ 
\hline 
1 & 0 & 1 & 0 & 1 & 1 & 1 \\ 
\hline 
1 & 0 & 0 & 0 & 1 & 1 & 1 \\ 
\hline 
0 & 1 & 1 & 1 & 1 & 0 & 1 \\ 
\hline 
0 & 1 & 0 & 1 & 0 & 0 & 0 \\ 
\hline 
0 & 0 & 1 & 1 & 1 & 0 & 1 \\ 
\hline 
0 & 0 & 0 & 1 & 0 & 0 & 0 \\ 
\hline 
\end{tabular}

Columns 5 and 7 are identical so they are logically equivalent. Also working with tables in Latex can be tricky\\

\hrulefill\\

\textbf{Question 8a:}

$\sum_{j=3}^6 (5j^2+(-1)^j) = \sum_{j=3}^6 (5j^2) + \sum_{j=3}^6 (-1)^j = (15^2+20^2+30^2)+ \sum_{j=0}^6 (-1)^j - \sum_{j=0}^2 (-1)^j $

$ = (15^2+20^2+30^2)+ (\frac{(-1)^7-1}{-1-1})- (\frac{(-1)^3-1}{-1-1})$\\

\textbf{8a. correction:}

I messed up the first sum and mutliplied first then squared.. and forgot j=6 in the sum $\sum_{j=3}^{6} 5j^2$

$5*(3^2+4^2+5^2+6^2)+(\frac{(-1)^7-1}{-1-1})- (\frac{(-1)^3-1}{-1-1})$ = 430+(0-0) = 430\\

\textbf{Question 8b:}

$\sum_{i=0}^8 (2^{i+1} - 3) = \sum_{i=0}^8 2^{i+1} - 8*3 = 2* \sum_{i=0}^8 2^i - 8*3$

$= 2*\frac{2^9-1}{2-1} - 24= 998$\\

\textbf{8b. correction}

I forgot to include i=0 on the sum: $\sum_{i=0}^{8} 3$ making it off by 3 so the answer should have been :

$2*\frac{2^9-1}{2-1} - 27 = 995$

\end{document}